break build but useful state_update def

theories/coneris/wp_update.v
@@ -201,7 +201,7 @@ Section wp_update.
     iApply HP. iFrame.
   Qed.
 
-  Global Instance is_except_0_pgl_wp E Q : IsExcept0 (wp_update E Q).
+  Global Instance is_except_0_wp_update E Q : IsExcept0 (wp_update E Q).
   Proof.
     by rewrite /IsExcept0 -{2}fupd_wp_update -except_0_fupd -fupd_intro.
   Qed.
@@ -238,3 +238,294 @@ Section wp_update.
 
 End wp_update.
 
+Section state_update.
+  Context `{!conerisGS Σ}.
+  Definition state_update_def E P:=
+    (∀ σ1 ε1,
+       state_interp σ1 ∗ err_interp ε1 ={E, ∅}=∗
+       state_step_coupl σ1 ε1 (λ σ2 ε2,
+                                 |={∅, E}=> state_interp σ2 ∗ err_interp ε2 ∗ P
+         )
+    )%I.
+  
+  Local Definition state_update_aux : seal (@state_update_def). Proof. by eexists. Qed.
+  Definition state_update := state_update_aux.(unseal).
+  Lemma state_update_unseal : state_update = state_update_def.
+  Proof. rewrite -state_update_aux.(seal_eq) //. Qed.
+
+  Lemma wp_update_state_update E P:
+    state_update E P -∗ wp_update E P.
+  Proof.
+    rewrite state_update_unseal/state_update_def.
+    iIntros.
+    by iApply wp_update_state_step_coupl.
+  Qed.
+
+  Lemma state_update_ret E P:
+    P -∗ state_update E P.
+  Proof. 
+    rewrite state_update_unseal/state_update_def.
+    iIntros.
+    iApply fupd_mask_intro; first set_solver.
+    iIntros "Hclose".
+    iApply state_step_coupl_ret.
+    iMod "Hclose".
+    iFrame. by iModIntro.
+  Qed.
+
+  Global Instance from_modal_state_update_state_update P E :
+    FromModal True modality_id (state_update E P) (state_update E P) P.
+  Proof. iIntros (_) "HP /=". by iApply state_update_ret. Qed.
+    
+  Lemma state_update_mono_fupd E1 E2 P:
+    E1 ⊆ E2 -> (|={E2,E1}=> state_update E1 (|={E1, E2}=> P)) -∗ state_update E2 P.
+  Proof.
+    rewrite state_update_unseal/state_update_def.
+    iIntros (Hsubseteq) "Hvs".
+    iIntros (σ1 ε1) "[H1 H2]".
+    iMod ("Hvs" with "[$]") as ">?".
+    iModIntro.
+    iApply (state_step_coupl_mono with "[][$]").
+    iIntros (??) ">(?&?&>?)". by iFrame.
+  Qed.
+
+  
+  Lemma state_update_mono E P Q:
+    (P={E}=∗Q) -∗ state_update E P -∗ state_update E Q.
+  Proof.
+    rewrite state_update_unseal/state_update_def.
+    iIntros "Hvs H".
+    iIntros (σ1 ε1) "[H1 H2]".
+    iMod ("H" with "[$]") as "?".
+    iModIntro.
+    iApply (state_step_coupl_mono with "[Hvs][$]").
+    iIntros (??) ">(?&?&?)".
+    iFrame.
+    by iApply "Hvs".
+  Qed.
+  
+  Lemma state_update_mono_fupd' E1 E2 P:
+    E1 ⊆ E2 -> (state_update E1 P) -∗ state_update E2 P.
+  Proof.
+    iIntros.
+    iApply state_update_mono_fupd; first done.
+    iApply fupd_mask_intro; first done.
+    iIntros "Hclose".
+    iApply (state_update_mono with "[Hclose][$]").
+    iIntros.
+    iModIntro.
+    by iMod "Hclose".
+  Qed.
+  
+  Lemma state_update_fupd E P:
+    (|={E}=> state_update E P) -∗ state_update E P.
+  Proof.
+    iIntros "H".
+    iApply state_update_mono_fupd; first done.
+    iMod "H".
+    iApply state_update_mono; last done.
+    by iIntros.
+  Qed.
+
+  Lemma state_update_fupd_change E1 E2 P Q:
+    (|={E1, E2}=> P) -∗ (P-∗ state_update E2 (|={E2, E1}=> Q)) -∗ state_update E1 Q.
+  Proof.
+    iIntros "H1 H2".
+    rewrite state_update_unseal/state_update_def.
+    iIntros (??) "[??]".
+    iMod "H1".
+    iMod ("H2" with "[$][$]") as "H2".
+    iModIntro.
+    iApply state_step_coupl_mono; last done.
+    simpl.
+    iIntros (??) ">(?&?&>?)".
+    by iFrame.
+  Qed.
+
+  Global Instance elim_modal_bupd_state_update p E P Q :
+    ElimModal True p false (|==> P) P (state_update E Q) (state_update E Q).
+  Proof.
+    intros ?.
+    rewrite bi.intuitionistically_if_elim/=.
+    iIntros "[H1 H2]".
+    iApply state_update_fupd.
+    iMod "H1".
+    iModIntro.
+    by iApply "H2".
+  Qed.
+  
+  Global Instance elim_modal_fupd_state_update p E1 E2 P Q :
+    ElimModal (True) p false
+            (|={E1,E2}=> P) P
+            (state_update E1 Q) (state_update E2 (|={E2, E1}=> Q)).
+  Proof.
+    intros ?.
+    rewrite bi.intuitionistically_if_elim/=.
+    iIntros "[??]".
+    iApply (state_update_fupd_change with "[$][$]").
+  Qed.
+  
+  Lemma state_update_bind E P Q:
+    state_update E P ∗ (P -∗ state_update E Q) ⊢ state_update E Q.
+  Proof.
+    rewrite state_update_unseal/state_update_def.
+    iIntros "[H1 H2]" (??) "[??]".
+    iMod ("H1" with "[$]") as "H1".
+    iModIntro.
+    iApply (state_step_coupl_bind with "[H2][$]").
+    iIntros (??) "H1".
+    iApply fupd_state_step_coupl.
+    iMod "H1" as "(?&?&?)".
+    by iMod ("H2" with "[$][$]").
+  Qed.
+
+  Global Instance elim_modal_state_update_state_update p E1 E2 P Q :
+    ElimModal (E1 ⊆ E2) p false (state_update E1 Q) Q (state_update E2 P) (state_update E2 P).
+  Proof.
+    iIntros (?) "[H1 H2]".
+    rewrite bi.intuitionistically_if_elim.
+    iApply state_update_mono_fupd; first exact.
+    iApply fupd_mask_intro; first exact; iIntros "Hclose".
+    iApply state_update_bind; iFrame.
+    iIntros.
+    iApply (state_update_fupd_change with "[$]").
+    iIntros.
+    iDestruct ("H2" with "[$]") as "H".
+    iApply (state_update_mono); last done.
+    iIntros.
+    iModIntro.
+    by iApply fupd_mask_intro_subseteq.
+  Qed.
+ 
+  Global Instance elim_modal_state_update_wp_update p E1 E2 P Q :
+    ElimModal (E1 ⊆ E2) p false (state_update E1 Q) Q (wp_update E2 P) (wp_update E2 P).
+  Proof.
+    (* rewrite state_update_unseal/state_update_def. *)
+    iIntros (?) "[H1 H2]".
+    iApply (wp_update_bind).
+    iFrame.
+    iApply wp_update_state_update.
+    iIntros.
+    iApply state_update_mono_fupd; first exact.
+    iApply fupd_mask_intro; first done.
+    iIntros "Hclose".
+    destruct p; simpl.
+    - iDestruct (bi.intuitionistically_elim with "[$]") as "H1".
+      iMod "H1".
+      iMod "Hclose" as "_".
+      iModIntro.
+      by iApply fupd_mask_intro_subseteq.
+    - iMod "H1".
+      iMod "Hclose" as "_".
+      iModIntro.
+      by iApply fupd_mask_intro_subseteq.
+  Qed.
+  
+  Global Instance elim_modal_state_update_wp e Φ p E1 E2 P :
+    ElimModal (E1 ⊆ E2) p false (state_update E1 P) P (WP e @ E2 {{ Φ }}) (WP e @ E2 {{ Φ }}).
+  Proof.
+    destruct p.
+    all: iIntros (?); simpl; iIntros "[H1 H2]".
+    1: iDestruct (bi.intuitionistically_elim with "[$]") as "H1".
+    all: iDestruct (state_update_mono_fupd with "[H1]") as "H1"; first exact;
+      last (iDestruct (wp_update_state_update with "[$]") as "H1"; iMod "H1"; by iApply "H2").
+    all: iApply fupd_mask_intro; first exact; iIntros "Hclose"; iMod "H1"; iModIntro; by iMod "Hclose".
+  Qed.
+
+  Lemma state_update_wp E P e Φ:
+    (state_update E P) -∗ (P -∗ WP e @ E {{Φ}}) -∗ WP e @ E {{Φ}}.
+  Proof.
+    iIntros ">? H".
+    by iApply "H".
+  Qed.
+
+  Global Instance is_except_0_state_update E Q : IsExcept0 (state_update E Q).
+  Proof.
+    rewrite /IsExcept0.
+    iIntros.
+    iApply (state_update_fupd E Q). by rewrite -except_0_fupd -fupd_intro.
+  Qed.
+
+  Lemma state_update_frame_l R E P :
+    R ∗ state_update E P ⊢ state_update E (P ∗ R).
+  Proof.
+    iIntros "[HR H]".
+    iMod "H".
+    iModIntro.
+    iFrame. 
+  Qed.
+
+  Global Instance frame_state_update p E R P Q:
+    Frame p R P Q → Frame p R (state_update E P) (state_update E Q).
+  Proof.
+    rewrite /Frame=> HR.
+    rewrite state_update_frame_l.
+    iIntros ">[??]".
+    iModIntro.
+    iApply HR; iFrame.
+  Qed.
+
+  Global Instance from_pure_bupd_state_update b E P φ :
+    FromPure b P φ → FromPure b (state_update E P) φ.
+  Proof.
+    rewrite /FromPure=> HP.
+    iIntros "H !>".
+    by iApply HP.
+  Qed.
+
+  Global Instance into_wand_state_update p q E R P Q :
+    IntoWand false false R P Q → IntoWand p q (state_update E R) (state_update E P) (state_update E Q).
+  Proof.
+    rewrite /IntoWand /= => HR.
+    rewrite !bi.intuitionistically_if_elim.
+    iIntros ">HR >HP !>". iApply (HR with "HR HP").
+  Qed.
+
+  Global Instance into_wand_bupd_persistent_state_update p q E R P Q :
+    IntoWand false q R P Q → IntoWand p q (state_update E R) P (state_update E Q).
+  Proof.
+    rewrite /IntoWand /= => HR. rewrite bi.intuitionistically_if_elim.
+    iIntros ">HR HP !>".
+    iApply (HR with "HR HP").
+  Qed.
+
+  Global Instance into_wand_bupd_args_state_update p q E R P Q :
+    IntoWand p false R P Q → IntoWand' p q R (state_update E P) (state_update E Q).
+  Proof.
+    rewrite /IntoWand' /IntoWand /= => ->.
+    rewrite bi.intuitionistically_if_elim.
+    iIntros "Hw HP".
+    iMod "HP".
+    iModIntro.
+    by iApply "Hw".
+  Qed.
+
+  Global Instance from_sep_bupd_state_update E P Q1 Q2 :
+    FromSep P Q1 Q2 → FromSep (state_update E P) (state_update E Q1) (state_update E Q2).
+  Proof.
+    rewrite /FromSep=> HP.
+    iIntros "[>HQ1 >HQ2] !>".
+    iApply HP. iFrame.
+  Qed.
+
+  Global Instance from_exist_state_update {B} P E (Φ : B → iProp Σ) :
+    FromExist P Φ → FromExist (state_update E P) (λ b, state_update E (Φ b))%I.
+  Proof.
+    rewrite /FromExist => HP.
+    iIntros "[%x >Hx] !>".
+    iApply HP. eauto.
+  Qed.
+
+  Global Instance into_forall_state_update {B} P E (Φ : B → iProp Σ) :
+    IntoForall P Φ → IntoForall (state_update E P) (λ b, state_update E (Φ b))%I.
+  Proof.
+    rewrite /IntoForall=>HP.
+    iIntros "> H" (b) "!>".
+    iApply (HP with "H").
+  Qed.
+
+  Global Instance from_assumption_state_update p E P Q :
+    FromAssumption p P Q → KnownRFromAssumption p P (state_update E Q).
+  Proof. rewrite /KnownRFromAssumption /FromAssumption=>->. iApply state_update_ret. Qed.
+  
+End state_update.
